

Tutorial 2 - Solution

Question 1

(a)

$$F\{y\} = \int_0^{\pi/2} (y^2 + y'^2 - 2y \sin x) dx, \quad y(0) = 0, \quad y(\pi/2) = 3/2.$$

The Euler-Lagrange equation gives

$$2y - 2 \sin x - \frac{d}{dx}(2y') = 0.$$

$$\Rightarrow y'' - y = -\sin x.$$

The solution to the homogeneous equation is

$$y_h = A \sinh x + B \cosh x.$$

Using the method of undetermined coefficients we have

$$\begin{aligned} y_p &= c_1 \sin x + c_2 \cos x \\ y_p'' &= -c_1 \sin x - c_2 \cos x. \end{aligned}$$

Substituting into the ODE we obtain

$$-c_1 \sin x - c_2 \cos x - c_1 \sin x - c_2 \cos x = -\sin x.$$

So $c_1 = 1/2$ and $c_2 = 0$. So the general solution is

$$y = A \sinh x + B \cosh x + \frac{1}{2} \sin x.$$

Now applying the end-point conditions

$$\begin{aligned} y(0) = 0 &\Rightarrow B = 0 \\ y(\pi/2) = 3/2 &\Rightarrow 3/2 = A \sinh(\pi/2) + 1/2 \\ &\Rightarrow A = \frac{1}{\sinh(\pi/2)}. \end{aligned}$$

So the solution to this problem is

$$y = \frac{\sinh x}{\sinh(\pi/2)} + \frac{1}{2} \sin x.$$

(b)

$$F\{y\} = \int_1^2 \frac{y'^2}{x^3} dx, \quad y(1) = 0, \quad y(2) = 15.$$

The functional is y -absent so it satisfies the equation

$$\begin{aligned} \frac{\partial f}{\partial y'} &= c \\ \frac{2y'}{x^3} &= c \\ y' &= \frac{c}{2} x^3. \end{aligned}$$

Integrating we obtain

$$y = \frac{c}{8} x^4 + d.$$

Now applying the end-point conditions

$$\begin{aligned} y(1) = 0 & \Rightarrow 0 = \frac{c}{8} + d \\ & \Rightarrow y = d(1 - x^4). \\ y(2) = 15 & \Rightarrow 15 = d(1 - 16) \\ & \Rightarrow d = -1. \end{aligned}$$

So the solution to this problem is

$$y = x^4 - 1.$$

(c)

$$F\{y\} = \int_0^2 (xy' + y'^2) dx, \quad y(0) = 1, \quad y(2) = 0.$$

Again the functional is y -absent so it satisfies the equation

$$\begin{aligned} \frac{\partial f}{\partial y'} &= c \\ x + 2y' &= c \\ y' &= \frac{c}{2} - \frac{x}{2}. \end{aligned}$$

Integrating we obtain

$$y = d + \frac{c}{2}x - \frac{x^2}{4}.$$

Now applying the end-point conditions

$$\begin{aligned} y(0) = 1 & \Rightarrow d = 1 \\ y(2) = 0 & \Rightarrow 0 = 1 + c - 1 \\ & \Rightarrow c = 0. \end{aligned}$$

So the solution to this problem is

$$y = 1 - \frac{x^2}{4}.$$

Question 2

Using Fermat's principle of least time, we want to design a material that gives circular arcs as optimal solutions to a variational problem. Following the notes we use the Calculus of Variations on the time functional

$$T\{y\} = \int \frac{\sqrt{1 + y'^2}}{c} dx,$$

but first let's convert to polar coordinates.

$$\begin{aligned} x = r \cos \theta & \Rightarrow \frac{dx}{d\theta} = \dot{r} \cos \theta - r \sin \theta, \\ y = r \sin \theta & \Rightarrow \frac{dy}{d\theta} = \dot{r} \sin \theta + r \cos \theta, \\ \text{and so } y' &= \frac{\dot{r} \sin \theta + r \cos \theta}{\dot{r} \cos \theta - r \sin \theta}. \end{aligned}$$

Note well that $y' = dy/dx$, and $\dot{r} = dr/d\theta$. So a short calculation yields

$$1 + y'^2 = \frac{\dot{r}^2 + r^2}{(\dot{r} \cos \theta - r \sin \theta)^2}.$$

Now the functional becomes

$$\begin{aligned} T\{y\} &= \int \frac{\sqrt{1+y'^2}}{c} dx \\ \Rightarrow T\{r\} &= \int \frac{\sqrt{\dot{r}^2 + r^2}}{c(\dot{r} \cos \theta - r \sin \theta)} (\dot{r} \cos \theta - r \sin \theta) d\theta \\ &= \int \frac{\sqrt{\dot{r}^2 + r^2}}{c} d\theta. \end{aligned}$$

Provided c does not depend explicitly on θ then this functional is θ -absent and therefore the extremal will satisfy

$$H = \dot{r} \frac{\partial f}{\partial \dot{r}} - f = \alpha, \quad \text{a constant.}$$

So let's assume that c is a function of r alone, that is $c = c(r)$, then

$$H = \dot{r} \frac{\dot{r}}{c(r)\sqrt{\dot{r}^2 + r^2}} - \frac{\sqrt{\dot{r}^2 + r^2}}{c(r)} = -\frac{r^2}{c(r)\sqrt{\dot{r}^2 + r^2}} = \alpha.$$

So solving for $c(r)$ we obtain

$$c(r) = -\frac{r^2}{\alpha\sqrt{\dot{r}^2 + r^2}}.$$

Now for a circular path we would require $\dot{r} = 0$ and therefore

$$c(r) = -\frac{r}{\alpha},$$

but how to find α ?

Question 3

The cone can be thought of as a surface in polar spherical coordinates

$$x = r \cos \theta \sin \phi, \quad y = r \sin \theta \sin \phi, \quad z = r \cos \phi,$$

where $\phi = \alpha$, a constant. So the surface is parameterised by

$$\mathbf{r}(r, \theta) = (r \cos \theta \sin \alpha, r \sin \theta \sin \alpha, r \cos \alpha).$$

Following the formulæ from lectures

$$\begin{aligned} P &= \left(\frac{\partial x}{\partial r}\right)^2 + \left(\frac{\partial y}{\partial r}\right)^2 + \left(\frac{\partial z}{\partial r}\right)^2 \\ &= \cos^2 \theta \sin^2 \alpha + \sin^2 \theta \sin^2 \alpha + \cos^2 \alpha = 1. \\ Q &= \frac{\partial x}{\partial r} \frac{\partial x}{\partial \theta} + \frac{\partial y}{\partial r} \frac{\partial y}{\partial \theta} + \frac{\partial z}{\partial r} \frac{\partial z}{\partial \theta} \\ &= -r \sin \theta \cos \theta \sin^2 \alpha + r \sin \theta \cos \theta \sin^2 \alpha + 0 = 0. \\ R &= \left(\frac{\partial x}{\partial \theta}\right)^2 + \left(\frac{\partial y}{\partial \theta}\right)^2 + \left(\frac{\partial z}{\partial \theta}\right)^2 \\ &= r^2 \sin^2 \theta \sin^2 \alpha + r^2 \cos^2 \theta \sin^2 \alpha + 0 = r^2 \sin^2 \alpha. \end{aligned}$$

So we can choose between either of the following formulations

$$L\{\theta(r)\} = \int_{r_0}^{r_1} \sqrt{1 + \theta'^2 r^2 \sin^2 \alpha} dr, \quad \text{or} \quad L\{r(\theta)\} = \int_{\theta_0}^{\theta_1} \sqrt{r'^2 + r^2 \sin^2 \alpha} d\theta.$$

Considering the second formulation we note that it is θ -absent (or autonomous) and therefore

$$H = r' \frac{\partial f}{\partial r'} - f = -c, \quad (\text{a constant}).$$

Therefore

$$\begin{aligned} \frac{r'^2}{\sqrt{r'^2 + r^2 \sin^2 \alpha}} - \sqrt{r'^2 + r^2 \sin^2 \alpha} &= -c \\ r^2 \sin^2 \alpha &= c \sqrt{r'^2 + r^2 \sin^2 \alpha} \\ r^4 \sin^4 \alpha &= c^2 (r'^2 + r^2 \sin^2 \alpha) \\ r^2 \sin^2 \alpha \left(\frac{r^2 \sin^2 \alpha}{c^2} - 1 \right) &= r'^2 \\ \frac{dr}{d\theta} &= r \sin \alpha \left(\frac{r^2 \sin^2 \alpha}{c^2} - 1 \right)^{1/2} \\ \frac{d\theta}{dr} &= \frac{1}{r \sin \alpha (r^2 \sin^2 \alpha / c^2 - 1)^{1/2}}. \end{aligned}$$

So integrating we have

$$\begin{aligned} \theta - d &= -\frac{1}{\sin \alpha} \tan^{-1} \left(\frac{1}{\sqrt{r^2 \sin^2 \alpha / c^2 - 1}} \right) \\ \sin \alpha (d - \theta) &= \tan^{-1} \left(\frac{1}{\sqrt{r^2 \sin^2 \alpha / c^2 - 1}} \right) \\ \tan(\sin \alpha (d - \theta)) &= \frac{1}{\sqrt{r^2 \sin^2 \alpha / c^2 - 1}} \\ \sqrt{r^2 \sin^2 \alpha / c^2 - 1} &= \cot(\sin \alpha (d - \theta)) \\ r^2 \sin^2 \alpha / c^2 &= 1 + \cot^2(\sin \alpha (d - \theta)) \\ r^2 \sin^2 \alpha / c^2 &= \csc^2(\sin \alpha (d - \theta)) \\ r \sin \alpha / c &= \csc(\sin \alpha (d - \theta)). \end{aligned}$$

Let's relabel our arbitrary constants $\mu = c / \sin \alpha$ and $\nu = d \sin \alpha$ then we have

$$r = \mu \csc(\nu - \theta \sin \alpha).$$

So we have a solution that has two arbitrary constants which we can resolve with the end-point conditions

$$r(\theta_0) = r_0, \quad \text{and} \quad r(\theta_1) = r_1.$$

Question 4

$$F\{y\} = \int_0^R \frac{x}{y'^2} dx.$$

This functional is y -absent and therefore the Euler-Lagrange equation is

$$\begin{aligned} \frac{\partial f}{\partial y'} &= \text{const} \\ -2 \frac{x}{y'^3} &= \text{const} \\ y'^3 &= -\frac{2x}{\text{const}} \\ y' &= \alpha x^{1/3}. \end{aligned}$$

So integrating

$$y = \frac{3\alpha}{4}x^{4/3} + \beta.$$

Now applying the end-point conditions

$$\begin{aligned} y(0) = L &\Rightarrow \beta = L, \\ y(R) = 0 &\Rightarrow 0 = \frac{3\alpha}{4}R^{4/3} + L, \\ &\Rightarrow \alpha = -\frac{4L}{3R^{4/3}}. \end{aligned}$$

$$\text{So } y = L \left[1 - \left(\frac{x}{R} \right)^{4/3} \right].$$

Lets assume $L = 1$, and $R = 1$ then

$$y = 1 + x^{4/3}, \quad y'^2 = \frac{16}{9}x^{2/3},$$

$$\text{So } F = \int_0^1 \frac{x}{1 + \frac{16}{9}x^{2/3}} dx \approx 0.2200 \dots,$$

but remember that this is not in the $L \gg R$ regime.

Question 5

(a)

If $f(y, y')$ does not explicitly depend on x then by the chain rule

$$\begin{aligned} \frac{df}{dx} &= \frac{\partial f}{\partial x} + \frac{\partial f}{\partial y} \frac{dy}{dx} + \frac{\partial f}{\partial y'} \frac{dy'}{dx} \\ &= y' f_y + y'' f_{y'} \\ \Rightarrow y' f_y &= \frac{df}{dx} - y'' f_{y'}. \end{aligned} \tag{1}$$

From the Euler-Lagrange equation

$$\begin{aligned} f_y - \frac{d}{dx} f_{y'} &= 0 \\ y' f_y - y' \frac{d}{dx} f_{y'} &= 0. \end{aligned}$$

and substitution from (1) yields

$$\frac{df}{dx} - y'' f_{y'} - y' \frac{d}{dx} f_{y'} = 0.$$

But the last two terms are a derivative of a product and therefore

$$\frac{df}{dx} - \frac{d}{dx} (y' f_{y'}) = 0,$$

and so integrating

$$f - y' f_{y'} = \text{const},$$

as required.

(b)

If $f(y, y', y'')$ does not explicitly depend on x then by the chain rule

$$\begin{aligned}\frac{df}{dx} &= \frac{\partial f}{\partial x} + \frac{\partial f}{\partial y} \frac{dy}{dx} + \frac{\partial f}{\partial y'} \frac{dy'}{dx} + \frac{\partial f}{\partial y''} \frac{dy''}{dx} \\ &= y' f_y + y'' f_{y'} + y''' f_{y''} \\ \Rightarrow y' f_y &= \frac{df}{dx} - y'' f_{y'} - y''' f_{y''}.\end{aligned}\tag{2}$$

From the Euler-Poisson equation

$$\begin{aligned}f_y - \frac{d}{dx} f_{y'} + \frac{d^2}{dx^2} f_{y''} &= 0 \\ y' f_y - y' \frac{d}{dx} f_{y'} + y' \frac{d^2}{dx^2} f_{y''} &= 0.\end{aligned}$$

and substitution from (2) yields

$$\frac{df}{dx} - y'' f_{y'} - y''' f_{y''} - y' \frac{d}{dx} f_{y'} + y' \frac{d^2}{dx^2} f_{y''} = 0.$$

But the second and fourth terms are a derivative of a product and therefore

$$\frac{df}{dx} - \frac{d}{dx} (y' f_{y'}) - y''' f_{y''} + y' \frac{d^2}{dx^2} f_{y''} = 0.$$

Now we add and subtract $y'' d/dx(f_{y''})$

$$\frac{df}{dx} - \frac{d}{dx} (y' f_{y'}) - y''' f_{y''} - y'' \frac{d}{dx} f_{y''} + y' \frac{d^2}{dx^2} f_{y''} + y'' \frac{d}{dx} f_{y''} = 0,$$

and now all the terms are also derivatives of products and so we obtain

$$\frac{df}{dx} - \frac{d}{dx} (y' f_{y'}) - \frac{d}{dx} (y'' f_{y''}) + \frac{d}{dx} \left(y' \frac{d}{dx} f_{y''} \right) = 0,$$

and so integrating

$$f - y' f_{y'} - y'' f_{y''} + y' \frac{d}{dx} f_{y''} = \text{const},$$

as required.